venom/passes/algebraic_opt/proofs/algebraicOptProofScript.sml
@@ -23,7 +23,7 @@ Theorem ao_transform_function_correct:
   !fuel ctx fn s.
     let fv' = ao_fn_total_fresh_vars fn in
     wf_function fn /\ wf_ssa fn /\ EVERY inst_wf (fn_insts fn) /\
-    ao_fresh_names_disjoint fn /\
+    ao_fresh_names_disjoint fn /\ dfg_block_local fn /\
     FDOM s.vs_vars = {} /\
     fn_entry_label fn = SOME s.vs_current_bb ==>
     (?e. run_blocks fuel ctx fn s = Error e) \/
